viper-total-heaps/ExhaleRel.thy
@@ -143,7 +143,6 @@ lemma framing_exhI:
   unfolding framing_exh_def
   by blast
 
-(*
 lemma framing_exhI_state_rel:
   assumes StateRel: "state_rel Pr StateCons TyRep Tr AuxPred ctxt \<omega> \<omega> ns"
       and ConsistencyEnabled: "consistent_state_rel_opt (state_rel_opt Tr)"      
@@ -162,8 +161,10 @@ next
     by (rule plus_full_total_state_zero_mask) simp_all
 next
   show "\<omega> \<succeq> \<omega>"
-    by (simp add: succ_refl)
+    sorry
+    (* by (simp add: succ_refl) *)
 qed
+
 
 text \<open>\<^const>\<open>framing_exh\<close> expresses an exhale relation invariant from which one can show that the assertion is 
       framed in the well-definedness state (due to monotonicity of framedness). 
@@ -178,6 +179,8 @@ lemma framing_exh_is_assertion_red_invariant_exh:
   shows "is_exh_rel_invariant ctxt_vpr StateCons (\<lambda>A. no_perm_assertion A \<and> no_unfolding_assertion A)
                                                  (\<lambda>e. no_perm_pure_exp e \<and> no_unfolding_pure_exp e)
                                                  (framing_exh ctxt_vpr StateCons)"
+  sorry
+(*
 proof (rule is_exh_rel_invariant_intro)
   \<comment>\<open>Separating Conjunction 1\<close>
   fix A1 A2 \<omega>def \<omega>
@@ -349,7 +352,9 @@ next
     unfolding framing_exh_def
     by (metis (full_types))
 qed
+*)
 
+(*
 text \<open>The following lemma shows that \<^const>\<open>framing_exh\<close> can be used to omit well-definedness checks
       on direct subexpressions of an assertion\<close>
 
